progress

alpha_map/Optional-lww_register/App_new_ts.fst
@@ -157,13 +157,13 @@ let relaxed_comm (s:concrete_st) (o1 o2 o3:op_t)
 let non_comm_help (o1 o2:op_t)
   : Lemma (requires distinct_ops o1 o2)
           (ensures (Set? (snd (snd o1)) \/ Set? (snd (snd o2)) ==> ~ (eq (do (do init_st o1) o2) (do (do init_st o2) o1)))) = ()
-          
+
 let non_comm (o1 o2:op_t)
   : Lemma (requires distinct_ops o1 o2)
           (ensures Either? (rc o1 o2) <==> commutes_with o1 o2) = 
   non_comm_help o1 o2
 
-let cond_comm (o1:op_t) (o2:op_t{distinct_ops o1 o2 /\ ~ (Either? (rc o1 o2)) /\ ~ (Ts_order? (rc o1 o2))}) (o3:op_t) = 
+let cond_comm (o1:op_t) (o2:op_t{distinct_ops o1 o2 /\ ~ (Either? (rc o1 o2)) (*/\ ~ (Ts_order? (rc o1 o2)*)}) (o3:op_t) = 
   if Unset? (snd (snd o3)) then true else false
 
 let cond_comm_base (s:concrete_st) (o1 o2 o3:op_t)
@@ -190,22 +190,29 @@ let rc_ind_right (l a b:concrete_st) (o1 o2' o2:op_t)
                     eq (merge l (do a o1) (do b o2)) (do (merge l (do a o1) b) o2))
           (ensures eq (merge l (do a o1) (do (do b o2') o2)) (do (merge l (do a o1) (do b o2')) o2)) = ()
 
-let rc_ind_left_l (l a b:concrete_st_l) (o1 o1' o2:(nat & (nat & op_l)))
-  : Lemma (requires eq_l (merge_l l (do_l a o1) (do_l b o2)) (do_l (merge_l l (do_l a o1) b) o2))
-          (ensures eq_l (merge_l l (do_l (do_l a o1') o1) (do_l b o2)) (do_l (merge_l l (do_l (do_l a o1') o1) b) o2)) = ()
-
-let rc_ind_left_e (l a b:concrete_st_e) (o1 o1' o2:(nat & (nat & op_e)))
-  : Lemma (requires fst o1 =!= fst o2 /\ Fst_then_snd? (rc_e o1 o2) /\
-                    eq_e (merge_e l (do_e a o1) (do_e b o2)) (do_e (merge_e l (do_e a o1) b) o2))
-          (ensures eq_e (merge_e l (do_e (do_e a o1') o1) (do_e b o2)) (do_e (merge_e l (do_e (do_e a o1') o1) b) o2)) = ()
+let rc_ind_right_base (l a b:concrete_st) (o1 o2' o2:op_t)
+  : Lemma (requires distinct_ops o1 o2 /\ Fst_then_snd? (rc o1 o2))
+          (ensures eq (merge l (do l o1) (do l o2)) (do (merge l (do l o1) l) o2)) = ()
           
+(*let ts_ind_right' (l a b:concrete_st) (o1 o2' o2:op_t)
+  : Lemma (requires distinct_ops o1 o2 /\ Ts_order? (rc o1 o2) /\
+                    eq (merge l (do a o1) (do b o2)) (do (merge l (do a o1) b) o2))
+          (ensures eq (merge l (do a o1) (do (do b o2') o2)) (do (merge l (do a o1) (do b o2')) o2)) = ()*)
+
 let rc_ind_left (l a b:concrete_st) (o1 o1' o2:op_t)
   : Lemma (requires distinct_ops o1 o2 /\ Fst_then_snd? (rc o1 o2) /\ 
                     eq (merge l (do a o1) (do b o2)) (do (merge l (do a o1) b) o2))
           (ensures eq (merge l (do (do a o1') o1) (do b o2)) (do (merge l (do (do a o1') o1) b) o2)) = 
-  rc_ind_left_l (fst l) (fst a) (fst b) (get_op_l o1) (get_op_l o1') (get_op_l o2);
-  rc_ind_left_e (snd l) (snd a) (snd b) (get_op_e o1) (get_op_e o1') (get_op_e o2)
+  assert (eq_e (snd (merge l (do a o1') (do b o2))) (snd (do (merge l (do a o1') b) o2))); //test - can be removed
+  assert (eq_e (snd (merge l (do (do a o1) o1') (do b o2))) (snd (do (merge l (do (do a o1) o1') b) o2))); //test - can be removed 
+  ()
 
+(*let ts_ind_left' (l a b:concrete_st) (o1 o1' o2:op_t)
+  : Lemma (requires distinct_ops o1 o2 /\ Ts_order? (rc o1 o2) /\ 
+                    (Fst_then_snd? (rc o1' o2) ==> eq (merge l (do a o1') (do b o2)) (do (merge l (do a o1') b) o2)) /\ //EXTRA!!
+                    eq (merge l (do a o1) (do b o2)) (do (merge l (do a o1) b) o2))
+          (ensures eq (merge l (do (do a o1') o1) (do b o2)) (do (merge l (do (do a o1') o1) b) o2)) = ()*)
+          
 //Special case of rc_intermediate_v1
 let rc_ind_lca (l:concrete_st) (ol o1 o2:op_t)
   : Lemma (requires distinct_ops o1 o2 /\ Fst_then_snd? (rc o1 o2) /\ distinct_ops ol o1 /\ distinct_ops ol o2 /\
@@ -216,47 +223,29 @@ let rc_base (o1 o2:op_t)
   : Lemma (requires distinct_ops o1 o2 /\ Fst_then_snd? (rc o1 o2))
           (ensures eq (merge init_st (do init_st o1) (do init_st o2)) (do (do init_st o1) o2)) = ()
 
-let rc_inter_base_right_l (l s1 s2 s3:concrete_st_l) (ob ol o1 o2:(nat & (nat & op_l))) 
-  : Lemma (requires eq_l (merge_l (do_l l ol) (do_l (do_l s1 ol) o1) (do_l (do_l s2 ol) o2)) (do_l (do_l (do_l s3 ol) o1) o2))
-          (ensures eq_l (merge_l (do_l l ol) (do_l (do_l s1 ol) o1) (do_l (do_l (do_l s2 ob) ol) o2)) 
-                        (do_l (do_l (do_l (do_l s3 ob) ol) o1) o2)) = ()
-
-let rc_inter_base_right_e1 (l s1 s2 s3:concrete_st_e) (ob ol o1 o2:(nat & (nat & op_e))) 
-  : Lemma (requires fst ob =!= fst ol /\ Fst_then_snd? (rc_e ob ol) /\
-                    fst o1 =!= fst o2 /\ Fst_then_snd? (rc_e o1 o2) /\
-                    eq_e (merge_e l (do_e s1 o1) (do_e s2 o2)) (do_e (do_e s3 o1) o2) /\
-               eq_e (merge_e (do_e l ol) (do_e (do_e s1 ol) o1) (do_e (do_e s2 ol) o2)) (do_e (do_e (do_e s3 ol) o1) o2) /\                 
-                    eq_e (merge_e l (do_e s1 ol) (do_e s2 ob)) (do_e (do_e s3 ob) ol))
-          (ensures eq_e (merge_e (do_e l ol) (do_e (do_e s1 ol) o1) (do_e (do_e (do_e s2 ob) ol) o2)) 
-                        (do_e (do_e (do_e (do_e s3 ob) ol) o1) o2)) = ()
-
-let rc_inter_base_right_e2 (l s1 s2 s3:concrete_st_e) (ob ol o1 o2:(nat & (nat & op_e))) 
-  : Lemma (requires fst ob =!= fst ol /\ Enable? (snd (snd ob)) /\ Enable? (snd (snd ol)) /\
-                    fst o1 =!= fst o2 /\ Fst_then_snd? (rc_e o1 o2) /\
-                    get_rid o2 = get_rid ob /\ //EXTRA!!
-                    eq_e (merge_e l (do_e s1 o1) (do_e s2 o2)) (do_e (do_e s3 o1) o2) /\
-               eq_e (merge_e (do_e l ol) (do_e (do_e s1 ol) o1) (do_e (do_e s2 ol) o2)) (do_e (do_e (do_e s3 ol) o1) o2) /\                 
-                    eq_e (merge_e l (do_e s1 ol) (do_e s2 ob)) (do_e (do_e s3 ob) ol))
-          (ensures eq_e (merge_e (do_e l ol) (do_e (do_e s1 ol) o1) (do_e (do_e (do_e s2 ob) ol) o2)) 
-                        (do_e (do_e (do_e (do_e s3 ob) ol) o1) o2)) = ()
-                        
-let rc_inter_base_right' (l s1 s2 s3:concrete_st) (ob ol o1 o2:op_t) 
-  : Lemma (requires distinct_ops ob ol /\ (Fst_then_snd? (rc ob ol) \/ (Ts_order? (rc ob ol) /\ fst ob < fst ol)) /\ 
-                    distinct_ops o1 o2 /\ Fst_then_snd? (rc o1 o2) /\
-                    get_rid o2 = get_rid ob /\ //EXTRA!!
+#push-options "--z3rlimit 300 --max_ifuel 3"
+let rc_inter_base_right'1 (l s1 s2 s3:concrete_st) (ob ol o1 o2:op_t) 
+  : Lemma (requires distinct_ops ob ol /\ Fst_then_snd? (rc ob ol) /\
+                    distinct_ops o1 o2 /\ Fst_then_snd? (rc o1 o2) /\ 
                     eq (merge l (do s1 o1) (do s2 o2)) (do (do s3 o1) o2) /\
                     eq (merge (do l ol) (do (do s1 ol) o1) (do (do s2 ol) o2)) (do (do (do s3 ol) o1) o2) /\                 
                     eq (merge l (do s1 ol) (do s2 ob)) (do (do s3 ob) ol))
-          (ensures eq (merge (do l ol) (do (do s1 ol) o1) (do (do (do s2 ob) ol) o2)) (do (do (do (do s3 ob) ol) o1) o2)) = 
-  rc_inter_base_right_l (fst l) (fst s1) (fst s2) (fst s3) (get_op_l ob) (get_op_l ol) (get_op_l o1) (get_op_l o2); 
-  if Fst_then_snd? (rc ob ol) then
-    rc_inter_base_right_e1 (snd l) (snd s1) (snd s2) (snd s3) (get_op_e ob) (get_op_e ol) (get_op_e o1) (get_op_e o2)
-  else rc_inter_base_right_e2 (snd l) (snd s1) (snd s2) (snd s3) (get_op_e ob) (get_op_e ol) (get_op_e o1) (get_op_e o2)
+          (ensures eq (merge (do l ol) (do (do s1 ol) o1) (do (do (do s2 ob) ol) o2)) (do (do (do (do s3 ob) ol) o1) o2)) = ()
 
-let rc_inter_base_left_l (l s1 s2 s3:concrete_st_l) (ob ol o1 o2:(nat & (nat & op_l))) 
-  : Lemma (requires eq_l (merge_l (do_l l ol) (do_l (do_l s1 ol) o1) (do_l (do_l s2 ol) o2)) (do_l (do_l (do_l s3 ol) o1) o2))
-          (ensures eq_l (merge_l (do_l l ol) (do_l (do_l (do_l s1 ob) ol) o1) (do_l (do_l s2 ol) o2)) 
-                        (do_l (do_l (do_l (do_l s3 ob) ol) o1) o2)) = ()
+let lo (o1 o2:op_t) =
+  (get_rid o1 = get_rid o2 /\ ~ (Either? (rc o1 o2)) /\ fst o1 < fst o2) \/
+  (get_rid o1 <> get_rid o2 /\ //~ (exists o3. get_rid o2 = get_rid o3 /\ ~ (Either? (rc o2 o3))) /\ 
+   (Fst_then_snd? (rc o1 o2) \/ Ts_order? (rc o1 o2)))
+  
+let rc_inter_base_right'2 (l s1 s2 s3:concrete_st) (ob ol o1 o2:op_t) 
+  : Lemma (requires distinct_ops ob ol /\ Ts_order? (rc ob ol) /\ fst ob < fst ol /\
+                    distinct_ops o1 o2 /\ Fst_then_snd? (rc o1 o2) /\ 
+                    get_rid o1 <> get_rid o2 /\ get_rid o1 <> get_rid ob /\ get_rid ob <> get_rid ol /\
+                    (Either? (rc ob o1) \/ lo ob o1) /\
+                    eq (merge l (do l o1) (do l o2)) (do (do l o1) o2) /\
+                    eq (merge (do l ol) (do (do l ol) o1) (do (do l ol) o2)) (do (do (do l ol) o1) o2) /\                 
+                    eq (merge l (do l ol) (do l ob)) (do (do l ob) ol))
+          (ensures eq (merge (do l ol) (do (do l ol) o1) (do (do (do l ob) ol) o2)) (do (do (do (do l ob) ol) o1) o2)) = ()
 
 let rc_inter_base_left_e1 (l s1 s2 s3:concrete_st_e) (ob ol o1 o2:(nat & (nat & op_e))) 
   : Lemma (requires fst ob =!= fst ol /\ Fst_then_snd? (rc_e ob ol) /\
@@ -282,95 +271,46 @@ let rc_inter_base_left' (l s1 s2 s3:concrete_st) (ob ol o1 o2:op_t)
                     eq (merge l (do s1 o1) (do s2 o2)) (do (do s3 o1) o2) /\
                     eq (merge (do l ol) (do (do s1 ol) o1) (do (do s2 ol) o2)) (do (do (do s3 ol) o1) o2) /\
                     eq (merge l (do s1 ob) (do s2 ol)) (do (do s3 ob) ol))
-          (ensures eq (merge (do l ol) (do (do (do s1 ob) ol) o1) (do (do s2 ol) o2)) (do (do (do (do s3 ob) ol) o1) o2)) = 
-  rc_inter_base_left_l (fst l) (fst s1) (fst s2) (fst s3) (get_op_l ob) (get_op_l ol) (get_op_l o1) (get_op_l o2); 
-  if Fst_then_snd? (rc ob ol) then
-    rc_inter_base_left_e1 (snd l) (snd s1) (snd s2) (snd s3) (get_op_e ob) (get_op_e ol) (get_op_e o1) (get_op_e o2)
-  else rc_inter_base_left_e2 (snd l) (snd s1) (snd s2) (snd s3) (get_op_e ob) (get_op_e ol) (get_op_e o1) (get_op_e o2)
+          (ensures eq (merge (do l ol) (do (do (do s1 ob) ol) o1) (do (do s2 ol) o2)) (do (do (do (do s3 ob) ol) o1) o2)) = ()
 
-let rc_inter_right_l (l s1 s2 s3:concrete_st_l) (o1 o2 ob ol o:(nat & (nat & op_l)))
-  : Lemma (requires eq_l (merge_l (do_l l ol) (do_l (do_l s1 ol) o1) (do_l (do_l (do_l s2 ob) ol) o2)) 
-                         (do_l (do_l (do_l (do_l s3 ob) ol) o1) o2))
-  (ensures eq_l (merge_l (do_l l ol) (do_l (do_l s1 ol) o1) (do_l (do_l (do_l (do_l s2 o) ob) ol) o2))
-                (do_l (do_l (do_l (do_l (do_l s3 o) ob) ol) o1) o2)) = ()
-
-let rc_inter_right_e1 (l s1 s2 s3:concrete_st_e) (o1 o2 ob ol o:(nat & (nat & op_e)))
-  : Lemma (requires fst ob =!= fst ol /\ Fst_then_snd? (rc_e ob ol) /\
-                    fst o1 =!= fst o2 /\ Fst_then_snd? (rc_e o1 o2) /\
-                    get_rid o <> get_rid ol (*o,ol must be concurrent*) /\
-                    //((~ (commutes_with_s o ob)) \/ Fst_then_snd? (rc_e o ol) \/ (Ts_order? (rc_e o ol) /\ fst o < fst ol)) /\
-                    eq_e (merge_e (do_e l ol) (do_e (do_e s1 ol) o1) (do_e (do_e (do_e s2 ob) ol) o2)) 
-                         (do_e (do_e (do_e (do_e s3 ob) ol) o1) o2))
-  (ensures eq_e (merge_e (do_e l ol) (do_e (do_e s1 ol) o1) (do_e (do_e (do_e (do_e s2 o) ob) ol) o2))
-                (do_e (do_e (do_e (do_e (do_e s3 o) ob) ol) o1) o2)) = () 
-
-let rc_inter_right_e2 (l s1 s2 s3:concrete_st_e) (o1 o2 ob ol o:(nat & (nat & op_e)))
-  : Lemma (requires fst ob =!= fst ol /\ Enable? (snd (snd ob)) /\ Enable? (snd (snd ol)) /\
-                    fst o1 =!= fst o2 /\ Fst_then_snd? (rc_e o1 o2) /\
-                    get_rid o <> get_rid ol (*o,ol must be concurrent*) /\
-                    (((Disable? (snd (snd o)) /\ Enable? (snd (snd ob))) \/ (Enable? (snd (snd o)) /\ Disable? (snd (snd ob))) \/
-                      (Enable? (snd (snd o)) /\ Enable? (snd (snd ob)))) \/
-                      Fst_then_snd? (rc_e o ol) \/ (Enable? (snd (snd o)) /\ Enable? (snd (snd ol)) /\ fst o < fst ol)) /\
-                    get_rid o = get_rid o2 /\ //EXTRA!!
-                    eq_e (merge_e (do_e l ol) (do_e (do_e s1 ol) o1) (do_e (do_e (do_e s2 ob) ol) o2)) 
-                         (do_e (do_e (do_e (do_e s3 ob) ol) o1) o2))
-  (ensures eq_e (merge_e (do_e l ol) (do_e (do_e s1 ol) o1) (do_e (do_e (do_e (do_e s2 o) ob) ol) o2))
-                (do_e (do_e (do_e (do_e (do_e s3 o) ob) ol) o1) o2)) = () 
-                
-let rc_inter_right' (l s1 s2 s3:concrete_st) (o1 o2 ob ol o:op_t)
+let rc_inter_right'1 (l s1 s2 s3:concrete_st) (o1 o2 ob ol o:op_t)
   : Lemma (requires distinct_ops o1 o2 /\ Fst_then_snd? (rc o1 o2) /\  
-                    distinct_ops ob ol /\ (Fst_then_snd? (rc ob ol) \/ (Ts_order? (rc ob ol) /\ fst ob < fst ol)) /\ 
-                    get_rid o = get_rid o2 /\ //EXTRA!!
+                    distinct_ops ob ol /\ Fst_then_snd? (rc ob ol) /\
                     get_rid o <> get_rid ol (*o,ol must be concurrent*) /\
+                    //get_rid o1 <> get_rid o2 /\ get_rid o1 <> get_rid ob /\ 
                     ((~ (commutes_with o ob)) \/ Fst_then_snd? (rc o ol) \/ (Ts_order? (rc o ol) /\ fst o < fst ol)) /\
                     eq (merge (do l ol) (do (do s1 ol) o1) (do (do (do s2 ob) ol) o2)) (do (do (do (do s3 ob) ol) o1) o2))
-  (ensures eq (merge (do l ol) (do (do s1 ol) o1) (do (do (do (do s2 o) ob) ol) o2)) (do (do (do (do (do s3 o) ob) ol) o1) o2)) = 
-  rc_inter_right_l (fst l) (fst s1) (fst s2) (fst s3) (get_op_l o1) (get_op_l o2) (get_op_l ob) (get_op_l ol) (get_op_l o); 
-  if Fst_then_snd? (rc ob ol) then
-    rc_inter_right_e1 (snd l) (snd s1) (snd s2) (snd s3) (get_op_e o1) (get_op_e o2) (get_op_e ob) (get_op_e ol) (get_op_e o)  
-  else rc_inter_right_e2 (snd l) (snd s1) (snd s2) (snd s3) (get_op_e o1) (get_op_e o2) (get_op_e ob) (get_op_e ol) (get_op_e o)
+  (ensures eq (merge (do l ol) (do (do s1 ol) o1) (do (do (do (do s2 o) ob) ol) o2)) (do (do (do (do (do s3 o) ob) ol) o1) o2)) = ()
 
-let rc_inter_left_l (l s1 s2 s3:concrete_st_l) (o1 o2 ob ol o:(nat & (nat & op_l)))
-  : Lemma (requires eq_l (merge_l (do_l l ol) (do_l (do_l (do_l s1 ob) ol) o1) (do_l (do_l s2 ol) o2)) 
-                         (do_l (do_l (do_l (do_l s3 ob) ol) o1) o2))
-  (ensures eq_l (merge_l (do_l l ol) (do_l (do_l (do_l (do_l s1 o) ob) ol) o1) (do_l (do_l s2 ol) o2))
-                (do_l (do_l (do_l (do_l (do_l s3 o) ob) ol) o1) o2)) = ()
-
-let rc_inter_left_e1 (l s1 s2 s3:concrete_st_e) (o1 o2 ob ol o:(nat & (nat & op_e)))
-  : Lemma (requires fst ob =!= fst ol /\ Fst_then_snd? (rc_e ob ol) /\
-                    fst o1 =!= fst o2 /\ Fst_then_snd? (rc_e o1 o2) /\
-                    get_rid o <> get_rid ol (*o,ol must be concurrent*) /\
-                    //((~ (commutes_with_s o ob)) \/ Fst_then_snd? (rc_e o ol) \/ (Ts_order? (rc_e o ol) /\ fst o < fst ol)) /\
-                    eq_e (merge_e (do_e l ol) (do_e (do_e (do_e s1 ob) ol) o1) (do_e (do_e s2 ol) o2)) 
-                         (do_e (do_e (do_e (do_e s3 ob) ol) o1) o2))
-  (ensures eq_e (merge_e (do_e l ol) (do_e (do_e (do_e (do_e s1 o) ob) ol) o1) (do_e (do_e s2 ol) o2))
-                (do_e (do_e (do_e (do_e (do_e s3 o) ob) ol) o1) o2)) = () 
-
-#push-options "--z3rlimit 300 --max_ifuel 3"
-let rc_inter_left_e2 (l s1 s2 s3:concrete_st_e) (o1 o2 ob ol o:(nat & (nat & op_e)))
-  : Lemma (requires fst ob =!= fst ol /\ Enable? (snd (snd ob)) /\ Enable? (snd (snd ol)) /\
-                    fst o1 =!= fst o2 /\ Fst_then_snd? (rc_e o1 o2) /\
-                    get_rid o <> get_rid ol (*o,ol must be concurrent*) /\
-                    (((Disable? (snd (snd o)) /\ Enable? (snd (snd ob))) \/ (Enable? (snd (snd o)) /\ Disable? (snd (snd ob))) \/
-                      (Enable? (snd (snd o)) /\ Enable? (snd (snd ob)))) \/
-                      Fst_then_snd? (rc_e o ol) \/ (Enable? (snd (snd o)) /\ Enable? (snd (snd ol)) /\ fst o < fst ol)) /\
-                    eq_e (merge_e (do_e l ol) (do_e (do_e (do_e s1 ob) ol) o1) (do_e (do_e s2 ol) o2)) 
-                         (do_e (do_e (do_e (do_e s3 ob) ol) o1) o2))
-  (ensures eq_e (merge_e (do_e l ol) (do_e (do_e (do_e (do_e s1 o) ob) ol) o1) (do_e (do_e s2 ol) o2))
-                (do_e (do_e (do_e (do_e (do_e s3 o) ob) ol) o1) o2)) = ()
-
-let rc_inter_left' (l s1 s2 s3:concrete_st) (o1 o2 ob ol o:op_t)
+let rc_inter_right'2 (l s1 s2 s3:concrete_st) (o1 o2 ob ol o:op_t)
   : Lemma (requires distinct_ops o1 o2 /\ Fst_then_snd? (rc o1 o2) /\  
-                    distinct_ops ob ol /\ (Fst_then_snd? (rc ob ol) \/ (Ts_order? (rc ob ol) /\ fst ob < fst ol)) /\ 
-                    get_rid o <> get_rid ol (*o,ol must be concurrent*) /\
+                    distinct_ops ob ol /\ Ts_order? (rc ob ol) /\ //get_rid ob <> get_rid ol /\
+                    //get_rid o <> get_rid ol (*o,ol must be concurrent*) /\
+                    get_rid o1 <> get_rid o2 /\ get_rid o1 <> get_rid ob /\
+                    (Either? (rc ob o1) \/ lo ob o1) /\
+                    (~ (commutes_with o ob) \/ Fst_then_snd? (rc o ol) \/ (Ts_order? (rc o ol) /\ fst o < fst ol)) /\
+                    eq (merge (do l ol) (do (do s1 ol) o1) (do (do (do s2 ob) ol) o2)) (do (do (do (do s3 ob) ol) o1) o2))
+  (ensures eq (merge (do l ol) (do (do s1 ol) o1) (do (do (do (do s2 o) ob) ol) o2)) (do (do (do (do (do s3 o) ob) ol) o1) o2)) = ()
+
+let rc_inter_left'1 (l s1 s2 s3:concrete_st) (o1 o2 ob ol o:op_t)
+  : Lemma (requires distinct_ops o1 o2 /\ Fst_then_snd? (rc o1 o2) /\  
+                    distinct_ops ob ol /\ Fst_then_snd? (rc ob ol) /\
+                    //get_rid o <> get_rid ol (*o,ol must be concurrent*) /\
+                    //get_rid o1 <> get_rid o2 /\ get_rid o1 <> get_rid ob /\ 
                     ((~ (commutes_with o ob)) \/ Fst_then_snd? (rc o ol) \/ (Ts_order? (rc o ol) /\ fst o < fst ol)) /\
                     eq (merge (do l ol) (do (do (do s1 ob) ol) o1) (do (do s2 ol) o2)) (do (do (do (do s3 ob) ol) o1) o2))
-  (ensures eq (merge (do l ol) (do (do (do (do s1 o) ob) ol) o1) (do (do s2 ol) o2)) (do (do (do (do (do s3 o) ob) ol) o1) o2)) = 
-  rc_inter_left_l (fst l) (fst s1) (fst s2) (fst s3) (get_op_l o1) (get_op_l o2) (get_op_l ob) (get_op_l ol) (get_op_l o); 
-  if Fst_then_snd? (rc ob ol) then
-    rc_inter_left_e1 (snd l) (snd s1) (snd s2) (snd s3) (get_op_e o1) (get_op_e o2) (get_op_e ob) (get_op_e ol) (get_op_e o)  
-  else rc_inter_left_e2 (snd l) (snd s1) (snd s2) (snd s3) (get_op_e o1) (get_op_e o2) (get_op_e ob) (get_op_e ol) (get_op_e o)
+      (ensures eq (merge (do l ol) (do (do (do (do s1 o) ob) ol) o1) (do (do s2 ol) o2)) (do (do (do (do (do s3 o) ob) ol) o1) o2)) = ()
 
+let rc_inter_left'2 (l s1 s2 s3:concrete_st) (o1 o2 ob ol o:op_t)
+  : Lemma (requires distinct_ops o1 o2 /\ Fst_then_snd? (rc o1 o2) /\  
+                    distinct_ops ob ol /\ Ts_order? (rc ob ol) /\
+                    //get_rid o <> get_rid ol (*o,ol must be concurrent*) /\
+                    get_rid o1 <> get_rid o2 /\ get_rid o1 <> get_rid ob /\ 
+                    (Either? (rc ob o1) \/ lo ob o1) /\
+                    ((~ (commutes_with o ob)) \/ Fst_then_snd? (rc o ol) \/ (Ts_order? (rc o ol) /\ fst o < fst ol)) /\
+                    eq (merge (do l ol) (do (do (do s1 ob) ol) o1) (do (do s2 ol) o2)) (do (do (do (do s3 ob) ol) o1) o2))
+      (ensures eq (merge (do l ol) (do (do (do (do s1 o) ob) ol) o1) (do (do s2 ol) o2)) (do (do (do (do (do s3 o) ob) ol) o1) o2)) = ()
+      
 let rc_inter_lca' (l s1 s2 s3:concrete_st) (o1 o2 ol oi:op_t)
   : Lemma (requires distinct_ops o1 o2 /\ Fst_then_snd? (rc o1 o2) /\ 
                     (exists o. Fst_then_snd? (rc o ol) \/ (Ts_order? (rc o ol) /\ fst o < fst ol)) /\ 
@@ -400,11 +340,12 @@ let ts_ind_left_e (l a b:concrete_st_e) (o1 o1' o2:(nat & (nat & op_e)))
           
 let ts_ind_left' (l a b:concrete_st) (o1 o1' o2:op_t)
   : Lemma (requires distinct_ops o1 o2 /\ Ts_order? (rc o1 o2) /\ fst o1 < fst o2 /\
+                    get_rid o1 <> get_rid o2 /\ get_rid o1' <> get_rid o2 /\
                     (Fst_then_snd? (rc o1' o2) ==> eq (merge l (do (do a o1) o1') (do b o2)) (do (merge l (do (do a o1) o1') b) o2)) /\ //EXTRA!! from rc_ind_left
                     eq (merge l (do a o1) (do b o2)) (do (merge l (do a o1) b) o2))
           (ensures eq (merge l (do (do a o1') o1) (do b o2)) (do (merge l (do (do a o1') o1) b) o2)) = 
-  ts_ind_left_l (fst l) (fst a) (fst b) (get_op_l o1) (get_op_l o1') (get_op_l o2);
-  ts_ind_left_e (snd l) (snd a) (snd b) (get_op_e o1) (get_op_e o1') (get_op_e o2)
+  ()//ts_ind_left_l (fst l) (fst a) (fst b) (get_op_l o1) (get_op_l o1') (get_op_l o2);
+  //ts_ind_left_e (snd l) (snd a) (snd b) (get_op_e o1) (get_op_e o1') (get_op_e o2)
 
 //Special case of rc_intermediate_v1
 let ts_ind_lca' (l:concrete_st) (ol o1 o2:op_t)
@@ -441,21 +382,26 @@ let ts_inter_base_right_e2 (l s1 s2 s3:concrete_st_e) (ob ol o1 o2:(nat & (nat &
           (ensures eq_e (merge_e (do_e l ol) (do_e (do_e s1 ol) o1) (do_e (do_e (do_e s2 ob) ol) o2)) 
                         (do_e (do_e (do_e (do_e s3 ob) ol) o1) o2)) = ()
                         
-let ts_inter_base_right' (l s1 s2 s3:concrete_st) (ob ol o1 o2:op_t) 
-  : Lemma (requires distinct_ops ob ol /\ (Fst_then_snd? (rc ob ol) \/ (Ts_order? (rc ob ol) /\ fst ob < fst ol)) /\ 
+let ts_inter_base_right'1 (l s1 s2 s3:concrete_st) (ob ol o1 o2:op_t) 
+  : Lemma (requires distinct_ops ob ol /\ Fst_then_snd? (rc ob ol) /\ 
                     distinct_ops o1 o2 /\ Ts_order? (rc o1 o2) /\ fst o1 < fst o2 /\
-                    //eq (merge l (do s1 o1) (do (do s2 ob) o2)) (do (do (merge l s1 (do s2 ob)) o2) o1) /\ //EXTRA!! comes from comm_ind_right
-                    //(Fst_then_snd? (rc ob ol) ==> eq (merge (do l ol) (do s1 ol) (do (do s2 ob) ol)) (do (do s3 ob) ol)) /\ //EXTRA!! comes from intermediate_base_zero_op
-                    (Fst_then_snd? (rc ob o1) ==> (eq (merge l (do s1 o1) (do s2 ob)) (do (merge l s1 (do s2 ob)) o1))) /\ //EXTRA!!
-                    eq (merge l (do s1 o1) (do s2 o2)) (do (do s3 o1) o2) /\
-                    eq (merge (do l ol) (do (do s1 ol) o1) (do (do s2 ol) o2)) (do (do (do s3 ol) o1) o2) /\
-                    eq (merge l (do s1 ol) (do s2 ob)) (do (do s3 ob) ol)) //***EXTRA***
-          (ensures eq (merge (do l ol) (do (do s1 ol) o1) (do (do (do s2 ob) ol) o2)) (do (do (do (do s3 ob) ol) o1) o2)) = 
-  ts_inter_base_right_l (fst l) (fst s1) (fst s2) (fst s3) (get_op_l ob) (get_op_l ol) (get_op_l o1) (get_op_l o2);
-  if Fst_then_snd? (rc ob ol) then
-    ts_inter_base_right_e1 (snd l) (snd s1) (snd s2) (snd s3) (get_op_e ob) (get_op_e ol) (get_op_e o1) (get_op_e o2)
-  else ts_inter_base_right_e2 (snd l) (snd s1) (snd s2) (snd s3) (get_op_e ob) (get_op_e ol) (get_op_e o1) (get_op_e o2)
+                    get_rid o1 <> get_rid o2 /\ get_rid o1 <> get_rid ob /\ 
+                    (Either? (rc ob o1) \/ lo ob o1) /\
+                    eq (merge l (do l o1) (do l o2)) (do (do l o1) o2) /\
+                    eq (merge (do l ol) (do (do l ol) o1) (do (do l ol) o2)) (do (do (do l ol) o1) o2) /\
+                    eq (merge l (do l ol) (do l ob)) (do (do l ob) ol)) //***EXTRA***
+          (ensures eq (merge (do l ol) (do (do l ol) o1) (do (do (do l ob) ol) o2)) (do (do (do (do l ob) ol) o1) o2)) = ()
 
+let ts_inter_base_right'2 (l s1 s2 s3:concrete_st) (ob ol o1 o2:op_t) 
+  : Lemma (requires distinct_ops ob ol /\ Ts_order? (rc ob ol) /\ 
+                    distinct_ops o1 o2 /\ Ts_order? (rc o1 o2) /\ fst o1 < fst o2 /\
+                    get_rid o1 <> get_rid o2 /\ get_rid o1 <> get_rid ob /\ 
+                    (Either? (rc ob o1) \/ lo ob o1) /\
+                    eq (merge l (do l o1) (do l o2)) (do (do l o1) o2) /\
+                    eq (merge (do l ol) (do (do l ol) o1) (do (do l ol) o2)) (do (do (do l ol) o1) o2) /\
+                    eq (merge l (do l ol) (do l ob)) (do (do l ob) ol)) //***EXTRA***
+          (ensures eq (merge (do l ol) (do (do l ol) o1) (do (do (do l ob) ol) o2)) (do (do (do (do l ob) ol) o1) o2)) = ()
+          
 let ts_inter_base_left_l (l s1 s2 s3:concrete_st_l) (ob ol o1 o2:(nat & (nat & op_l))) 
   : Lemma (requires eq_l (merge_l (do_l l ol) (do_l (do_l s1 ol) o1) (do_l (do_l s2 ol) o2)) (do_l (do_l (do_l s3 ol) o1) o2))
           (ensures eq_l (merge_l (do_l l ol) (do_l (do_l (do_l s1 ob) ol) o1) (do_l (do_l s2 ol) o2)) 
@@ -480,19 +426,25 @@ let ts_inter_base_left_e2 (l s1 s2 s3:concrete_st_e) (ob ol o1 o2:(nat & (nat & 
           (ensures eq_e (merge_e (do_e l ol) (do_e (do_e (do_e s1 ob) ol) o1) (do_e (do_e s2 ol) o2)) 
                         (do_e (do_e (do_e (do_e s3 ob) ol) o1) o2)) = ()
 
-let ts_inter_base_left' (l s1 s2 s3:concrete_st) (ob ol o1 o2:op_t) 
-  : Lemma (requires distinct_ops ob ol /\ (Fst_then_snd? (rc ob ol) \/ (Ts_order? (rc ob ol) /\ fst ob < fst ol)) /\ 
+let ts_inter_base_left'1 (l s1 s2 s3:concrete_st) (ob ol o1 o2:op_t) 
+  : Lemma (requires distinct_ops ob ol /\ Fst_then_snd? (rc ob ol) /\ 
                     distinct_ops o1 o2 /\ Ts_order? (rc o1 o2) /\ fst o1 < fst o2 /\
-                    //eq (merge l (do (do s1 ob) o1) (do s2 o2)) (do (do (merge l (do s1 ob) s2) o2) o1) /\ //EXTRA!! comes from comm_ind_right
-                    (Fst_then_snd? (rc ob o2) ==> eq (merge l (do s1 ob) (do s2 o2)) (do (merge l (do s1 ob) s2) o2)) /\ //EXTRA!!
-                    eq (merge l (do s1 o1) (do s2 o2)) (do (do s3 o1) o2) /\
-                    eq (merge (do l ol) (do (do s1 ol) o1) (do (do s2 ol) o2)) (do (do (do s3 ol) o1) o2) /\
-                    eq (merge l (do s1 ob) (do s2 ol)) (do (do s3 ob) ol)) //***EXTRA***
-          (ensures eq (merge (do l ol) (do (do (do s1 ob) ol) o1) (do (do s2 ol) o2)) (do (do (do (do s3 ob) ol) o1) o2)) = 
-  ts_inter_base_left_l (fst l) (fst s1) (fst s2) (fst s3) (get_op_l ob) (get_op_l ol) (get_op_l o1) (get_op_l o2);
-  if Fst_then_snd? (rc ob ol) then
-    ts_inter_base_left_e1 (snd l) (snd s1) (snd s2) (snd s3) (get_op_e ob) (get_op_e ol) (get_op_e o1) (get_op_e o2)
-  else ts_inter_base_left_e2 (snd l) (snd s1) (snd s2) (snd s3) (get_op_e ob) (get_op_e ol) (get_op_e o1) (get_op_e o2)
+                    get_rid o1 <> get_rid o2 /\ get_rid o1 <> get_rid ob /\ 
+                    (Either? (rc ob o1) \/ lo ob o1) /\
+                    eq (merge l (do l o1) (do l o2)) (do (do l o1) o2) /\
+                    eq (merge (do l ol) (do (do l ol) o1) (do (do l ol) o2)) (do (do (do l ol) o1) o2) /\
+                    eq (merge l (do l ob) (do l ol)) (do (do l ob) ol)) //***EXTRA***
+          (ensures eq (merge (do l ol) (do (do (do l ob) ol) o1) (do (do l ol) o2)) (do (do (do (do l ob) ol) o1) o2)) = ()
+
+let ts_inter_base_left'2 (l s1 s2 s3:concrete_st) (ob ol o1 o2:op_t) 
+  : Lemma (requires distinct_ops ob ol /\ Ts_order? (rc ob ol) /\ 
+                    distinct_ops o1 o2 /\ Ts_order? (rc o1 o2) /\ fst o1 < fst o2 /\
+                    get_rid o1 <> get_rid o2 /\ get_rid o1 <> get_rid ob /\ 
+                    (Either? (rc ob o1) \/ lo ob o1) /\
+                    eq (merge l (do l o1) (do l o2)) (do (do l o1) o2) /\
+                    eq (merge (do l ol) (do (do l ol) o1) (do (do l ol) o2)) (do (do (do l ol) o1) o2) /\
+                    eq (merge l (do l ob) (do l ol)) (do (do l ob) ol)) //***EXTRA***
+          (ensures eq (merge (do l ol) (do (do (do l ob) ol) o1) (do (do l ol) o2)) (do (do (do (do l ob) ol) o1) o2)) = ()
 
 let ts_inter_right_l (l s1 s2 s3:concrete_st_l) (o1 o2 ob ol o:(nat & (nat & op_l)))
   : Lemma (requires eq_l (merge_l (do_l l ol) (do_l (do_l s1 ol) o1) (do_l (do_l (do_l s2 ob) ol) o2)) 
@@ -526,18 +478,86 @@ let ts_inter_right_e2 (l s1 s2 s3:concrete_st_e) (o1 o2 ob ol o:(nat & (nat & op
       (ensures eq_e (merge_e (do_e l ol) (do_e (do_e s1 ol) o1) (do_e (do_e (do_e (do_e s2 o) ob) ol) o2)) 
                     (do_e (do_e (do_e (do_e (do_e s3 o) ob) ol) o1) o2)) = ()
                     
-let ts_inter_right' (l s1 s2 s3:concrete_st) (o1 o2 ob ol o:op_t)
+let ts_inter_right'1 (l s1 s2 s3:concrete_st) (o1 o2 ob ol o:op_t)
   : Lemma (requires distinct_ops o1 o2 /\ Ts_order? (rc o1 o2) /\ fst o1 < fst o2 /\
-                    distinct_ops ob ol /\ (Fst_then_snd? (rc ob ol) \/ (Ts_order? (rc ob ol) /\ fst ob < fst ol)) /\ 
-                    get_rid o <> get_rid ol /\ get_rid o2 = get_rid ob /\ get_rid o = get_rid o2 /\ get_rid o1 <> get_rid o2 /\ //EXTRA!!
-                    distinct_ops o ol /\ Either? (rc o ol) /\ //EXTRA!!
+                    distinct_ops ob ol /\ Fst_then_snd? (rc ob ol) /\
+                    //get_rid o <> get_rid ol /\ 
+                    get_rid o1 <> get_rid o2 /\ get_rid o1 <> get_rid ob /\ 
+                    (Either? (rc ob o1) \/ lo ob o1) /\
+                    //distinct_ops o ol /\ Either? (rc o ol) /\ //EXTRA!!
                     ((~ (commutes_with o ob)) \/ Fst_then_snd? (rc o ol) \/ (Ts_order? (rc o ol) /\ fst o < fst ol)) /\
                     eq (merge (do l ol) (do (do s1 ol) o1) (do (do (do s2 ob) ol) o2)) (do (do (do (do s3 ob) ol) o1) o2))
-      (ensures eq (merge (do l ol) (do (do s1 ol) o1) (do (do (do (do s2 o) ob) ol) o2)) (do (do (do (do (do s3 o) ob) ol) o1) o2)) =
-  ts_inter_right_l (fst l) (fst s1) (fst s2) (fst s3) (get_op_l o1) (get_op_l o2) (get_op_l ob) (get_op_l ol) (get_op_l o);
-  if Fst_then_snd? (rc ob ol) then
-    ts_inter_right_e1 (snd l) (snd s1) (snd s2) (snd s3) (get_op_e o1) (get_op_e o2) (get_op_e ob) (get_op_e ol) (get_op_e o)
-  else ts_inter_right_e2 (snd l) (snd s1) (snd s2) (snd s3) (get_op_e o1) (get_op_e o2) (get_op_e ob) (get_op_e ol) (get_op_e o)
+      (ensures eq (merge (do l ol) (do (do s1 ol) o1) (do (do (do (do s2 o) ob) ol) o2)) (do (do (do (do (do s3 o) ob) ol) o1) o2)) = ()
+
+let lo' (o1 o2:op_t) =
+  (get_rid o1 = get_rid o2 /\ fst o1 < fst o2 /\ ~ (Either? (rc o1 o2))) \/
+  (get_rid o1 <> get_rid o2 /\ ~ (exists o3. fst o2 < fst o3 /\ get_rid o2 = get_rid o3 /\ ~ (Either? (rc o2 o3))) /\ 
+   (Fst_then_snd? (rc o1 o2) \/ (Ts_order? (rc o1 o2) /\ fst o1 < fst o2)))
+
+let lo_mod (o1 o2 o3:op_t) =
+  (get_rid o1 = get_rid o2 /\ ~ (Either? (rc o1 o2))) \/
+  (get_rid o1 <> get_rid o2 /\ ~ (get_rid o2 = get_rid o3 /\ ~ (Either? (rc o2 o3))) /\ 
+   (Fst_then_snd? (rc o1 o2) \/ Ts_order? (rc o1 o2)))
+
+#set-options "--z3rlimit 500 --ifuel 5"
+let ts_inter_right' (l s1 s2 s3:concrete_st) (o1 o2 ob ol o:op_t)
+  : Lemma (requires distinct_ops o1 o2 /\ Ts_order? (rc o1 o2) /\ fst o1 < fst o2 /\
+                    distinct_ops ob ol /\ Ts_order? (rc ob ol) /\ fst ob < fst ol /\ get_rid ob <> get_rid ol /\
+                    get_rid o <> get_rid ol (*o,ol must be concurrent*) /\
+                    get_rid o1 <> get_rid ob /\ get_rid o1 <> get_rid o2 /\ get_rid o <> get_rid o1 /\ //EXTRA!!
+                    Set? (snd (snd o)) /\
+                    (Either? (rc o o1) \/ lo o o1) /\
+                    (Either? (rc o o2) \/ lo o o2) /\
+                    (Either? (rc ob o1) \/ lo ob o1) /\
+                    (Either? (rc ob o2) \/ lo ob o2) /\
+                    (Either? (rc ol o1) \/ lo ol o1) /\
+                    (Either? (rc ol o2) \/ lo ol o2) /\
+                    (Either? (rc o ob) \/ lo' o ob) /\
+                    (Either? (rc o ol) \/ lo' o ol) /\
+                    (Either? (rc ob ol) \/ lo' ob ol) /\
+                    //get_rid o2 = get_rid ob /\
+                    eq (merge (do l ol) (do (do l ol) o1) (do (do (do (do l o) ob) ol) o2)) (do (do (do (do (do l o) ob) ol) o1) o2) /\
+                    ((Fst_then_snd? (rc o1 o2) \/ Either? (rc o1 o2)) ==> eq (merge (do l ol) (do (do s1 ol) o1) (do (do (do (do s2 o) ob) ol) o2)) (do (do (do (do (do s3 o) ob) ol) o1) o2) /\
+                    eq (merge (do l ol) (do (do s1 ol) o1) (do (do (do s2 o) ob) ol)) (do (do (do (do s3 o) ob) ol) o1) /\
+                    eq (merge (do l ol) (do s1 ol) (do (do (do s2 o) ob) ol)) (do (do (do s3 o) ob) ol) /\
+                    eq (merge (do l ol) (do s1 ol) (do (do s2 ob) ol)) (do (do s3 ob) ol) /\
+                    eq (merge l s1 (do (do s2 o1) o2)) (do (merge l s1 (do s2 o1)) o2) /\
+                    eq (merge l (do (do s1 o1) o2) s2) (do (merge l (do s1 o1) s2) o2) /\
+                    eq (merge (do l ol) (do (do s2 ol) o1) (do (do (do (do s1 o) ob) ol) o2)) (do (do (do (do (do s3 o) ob) ol) o1) o2)) /\
+                    eq (merge l (do s1 o1) (do (do s2 ob) o2)) (do (merge l (do s1 o1) (do s2 ob)) o2) /\               
+                    ((~ (commutes_with o ob)) \/ Fst_then_snd? (rc o ol) \/ (Ts_order? (rc o ol) /\ fst o < fst ol)) /\
+                    eq (merge (do l ol) (do (do s1 ol) o1) (do (do (do s2 ob) ol) o2)) (do (do (do (do s3 ob) ol) o1) o2))
+      (ensures eq_e (snd (merge (do l ol) (do (do s1 ol) o1) (do (do (do (do s2 o) ob) ol) o2))) (snd (do (do (do (do (do s3 o) ob) ol) o1) o2))) = admit()
+
+#set-options "--z3rlimit 500 --ifuel 5"
+let ts_inter_right'2 (l s1 s2 s3:concrete_st) (o1 o2 ob ol o:op_t)
+  : Lemma (requires distinct_ops o1 o2 /\ Ts_order? (rc o1 o2) /\ fst o1 < fst o2 /\
+                    distinct_ops ob ol /\ Ts_order? (rc ob ol) /\ fst ob < fst ol /\ get_rid ob <> get_rid ol /\ 
+                    get_rid o <> get_rid ol (*o,ol must be concurrent*) /\
+                    get_rid o1 <> get_rid o2 /\ get_rid o1 <> get_rid ob /\ get_rid o1 <> get_rid o /\
+                    (Either? (rc ob o1) \/ lo ob o1) /\ (Either? (rc ob o2) \/ lo ob o2) /\
+                    (Either? (rc ol o1) \/ lo ol o1) /\ (Either? (rc ol o2) \/ lo ol o2) /\
+                    (Either? (rc o o1) \/ lo o o1) /\ (Either? (rc o o2) \/ lo o o2) /\
+                    eq (merge l (do s1 o1) (do s2 o2)) (do (do s3 o1) o2) /\
+                    eq_e (snd (merge l (do s1 o2) (do s2 o1))) (snd (do (do s3 o1) o2)) /\
+                    eq (merge (do l ol) (do (do s1 ol) o1) (do (do s2 ol) o2)) (do (do (do s3 ol) o1) o2) /\
+                    eq (merge l (do s1 ol) (do s2 ob)) (do (do s3 ob) ol) /\
+                    eq_e (snd (merge l (do s1 ob) (do s2 ol))) (snd (do (do s3 ob) ol)) /\
+                    eq (merge l (do s1 o1) (do (do s2 o) o2)) (do (merge l (do s1 o1) (do s2 o)) o2) /\
+                    eq (merge l (do s1 o1) (do (do s2 ob) o2)) (do (merge l (do s1 o1) (do s2 ob)) o2) /\
+                    eq (merge l (do s1 o1) (do (do s2 ol) o2)) (do (merge l (do s1 o1) (do s2 ol)) o2) /\
+                    (~ (Either? (rc o ob)) \/ Fst_then_snd? (rc o ol) \/ (Ts_order? (rc o ol) /\ fst o < fst ol)) /\
+                    eq (merge (do l o2) (do (do s1 o2) ob) (do (do (do s2 o1) o2) ol)) (do (do (do (do s3 o1) o2) ob) ol) /\
+                    eq (merge (do l ol) (do (do s1 ol) o1) (do (do (do s2 ob) ol) o2)) (do (do (do (do s3 ob) ol) o1) o2) )
+      (ensures eq_e (snd (merge (do l ol) (do (do s1 ol) o1) (do (do (do (do s2 o) ob) ol) o2))) (snd (do (do (do (do (do s3 o) ob) ol) o1) o2))) = admit();
+  (*if Set? (snd (snd o)) && get_rid o = get_rid o2 && get_rid ob = get_rid o2 then admit() //done
+  else if Set? (snd (snd o)) && get_rid o = get_rid o2 && get_rid ob <> get_rid o2 then admit() //done
+  else*) if Set? (snd (snd o)) && get_rid o <> get_rid o2 && get_rid ob = get_rid o2 then () //not done
+  (*else if Set? (snd (snd o)) && get_rid o <> get_rid o2 && get_rid ob <> get_rid o2 then admit() //not done
+  else if Unset? (snd (snd o)) && get_rid o = get_rid o2 && get_rid ob = get_rid o2 then admit() //not done
+  else if Unset? (snd (snd o)) && get_rid o = get_rid o2 && get_rid ob <> get_rid o2 then admit() //not done
+  else if Unset? (snd (snd o)) && get_rid o <> get_rid o2 && get_rid ob = get_rid o2 then admit()*) //not done
+  else admit() //not done
 
 let ts_inter_left_l (l s1 s2 s3:concrete_st_l) (o1 o2 ob ol o:(nat & (nat & op_l)))
   : Lemma (requires eq_l (merge_l (do_l l ol) (do_l (do_l (do_l s1 ob) ol) o1) (do_l (do_l s2 ol) o2)) 
@@ -557,19 +577,42 @@ let ts_inter_left_e1 (l s1 s2 s3:concrete_st_e) (o1 o2 ob ol o:(nat & (nat & op_
       (ensures eq_e (merge_e (do_e l ol) (do_e (do_e (do_e (do_e s1 o) ob) ol) o1) (do_e (do_e s2 ol) o2)) 
                     (do_e (do_e (do_e (do_e (do_e s3 o) ob) ol) o1) o2)) = ()
 
-let ts_inter_left' (l s1 s2 s3:concrete_st) (o1 o2 ob ol o:op_t)
-  : Lemma (requires distinct_ops o1 o2 /\ Ts_order? (rc o1 o2) /\ fst o1 < fst o2 /\ 
-                    distinct_ops ob ol /\ (Fst_then_snd? (rc ob ol) \/ (Ts_order? (rc ob ol) /\ fst ob < fst ol)) /\ 
-                    //get_rid o <> get_rid ol (*o,ol must be concurrent*) /\
-                    distinct_ops o ol /\ Either? (rc o ol) /\ //EXTRA!!
+let ts_inter_left'1 (l s1 s2 s3:concrete_st) (o1 o2 ob ol o:op_t)
+  : Lemma (requires distinct_ops o1 o2 /\ Ts_order? (rc o1 o2) /\ fst o1 < fst o2 /\
+                    distinct_ops ob ol /\ Fst_then_snd? (rc ob ol) /\
+                    //get_rid o <> get_rid ol /\ 
+                    get_rid o1 <> get_rid o2 /\ get_rid o1 <> get_rid ob /\ 
+                    (Either? (rc ob o1) \/ lo ob o1) /\
+                    //distinct_ops o ol /\ Either? (rc o ol) /\ //EXTRA!!
                     ((~ (commutes_with o ob)) \/ Fst_then_snd? (rc o ol) \/ (Ts_order? (rc o ol) /\ fst o < fst ol)) /\
                     eq (merge (do l ol) (do (do (do s1 ob) ol) o1) (do (do s2 ol) o2)) (do (do (do (do s3 ob) ol) o1) o2))
-      (ensures eq (merge (do l ol) (do (do (do (do s1 o) ob) ol) o1) (do (do s2 ol) o2)) (do (do (do (do (do s3 o) ob) ol) o1) o2)) =
-  ts_inter_left_l (fst l) (fst s1) (fst s2) (fst s3) (get_op_l o1) (get_op_l o2) (get_op_l ob) (get_op_l ol) (get_op_l o);
-  if Fst_then_snd? (rc ob ol) then
-    ts_inter_left_e1 (snd l) (snd s1) (snd s2) (snd s3) (get_op_e o1) (get_op_e o2) (get_op_e ob) (get_op_e ol) (get_op_e o)
-  else ()
+      (ensures eq (merge (do l ol) (do (do (do (do s1 o) ob) ol) o1) (do (do s2 ol) o2)) (do (do (do (do (do s3 o) ob) ol) o1) o2)) = ()
 
+#set-options "--z3rlimit 500 --ifuel 5"
+let ts_inter_left'2 (l s1 s2 s3:concrete_st) (o1 o2 ob ol o:op_t)
+  : Lemma (requires distinct_ops o1 o2 /\ Ts_order? (rc o1 o2) /\ fst o1 < fst o2 /\
+                    distinct_ops ob ol /\ Ts_order? (rc ob ol) /\ fst ob < fst ol /\
+                    //get_rid o <> get_rid ol /\ 
+                    get_rid o1 <> get_rid o2 /\ get_rid o1 <> get_rid ob /\ 
+                    (Either? (rc ob o1) \/ lo ob o1) /\
+                    (Either? (rc ol o1) \/ lo ol o1) /\
+                    (Either? (rc o o1) \/ lo o o1) /\
+                    (Either? (rc ob o2) \/ lo ob o2) /\
+                    (Either? (rc ol o2) \/ lo ol o2) /\
+                    (Either? (rc o o2) \/ lo o o2) /\
+                    eq (merge (do l ol) (do (do (do s1 ob) ol) o1) (do s2 ol)) (do (do (do s3 ob) ol) o1) /\ //EXTRA!! comes from one_op_inter_base_right'
+                    eq (merge (do l ol) (do (do (do s1 ob) ol) o2) (do s2 ol)) (do (do (do s3 ob) ol) o2) /\ //EXTRA!! comes from one_op_inter_base_right'
+                    eq (merge (do l ol) (do (do (do s1 ob) ol) o) (do s2 ol)) (do (do (do s3 ob) ol) o) /\ //EXTRA!! comes from one_op_inter_base_right'
+                    (Fst_then_snd? (rc o1 o2) ==> eq (merge (do l ol) (do (do (do (do s1 o) ob) ol) o1) (do (do s2 ol) o2)) (do (do (do (do (do s3 o) ob) ol) o1) o2)) /\
+                    eq (merge l (do l o1) (do l o2)) (do (do l o1) o2) /\
+                    eq (merge (do l ol) (do (do l ol) o1) (do (do l ol) o2)) (do (do (do l ol) o1) o2) /\
+                    eq (merge l (do l ob) (do l ol)) (do (do l ob) ol) /\
+                    eq (merge (do l ol) (do (do (do (do l o) ob) ol) o1) (do (do l ol) o2)) (do (do (do (do (do l o) ob) ol) o1) o2) /\
+                    //distinct_ops o ol /\ Either? (rc o ol) /\ //EXTRA!!
+                    ((~ (commutes_with o ob)) \/ Fst_then_snd? (rc o ol) \/ (Ts_order? (rc o ol) /\ fst o < fst ol)) /\
+                    eq (merge (do l ol) (do (do (do s1 ob) ol) o1) (do (do s2 ol) o2)) (do (do (do (do s3 ob) ol) o1) o2))
+      (ensures eq (merge (do l ol) (do (do (do (do s1 o) ob) ol) o1) (do (do s2 ol) o2)) (do (do (do (do (do s3 o) ob) ol) o1) o2)) = admit()
+      
 let ts_inter_lca' (l s1 s2 s3:concrete_st) (o1 o2 ol oi:op_t)
   : Lemma (requires distinct_ops o1 o2 /\ Ts_order? (rc o1 o2) /\ fst o1 < fst o2 /\
                     (exists o. Fst_then_snd? (rc o ol) \/ (Ts_order? (rc o ol) /\ fst o < fst ol)) /\ 
@@ -612,6 +655,35 @@ let one_op_inter_base_left' (l s1 s2 s3:concrete_st) (ob ol o1:op_t)
           (ensures eq (merge (do l ol) (do (do s1 ob) ol) (do (do s2 ol) o1)) (do (do (do s3 ob) ol) o1)) = () //done
 
 let one_op_inter_right'1 (l s1 s2 s3:concrete_st) (o1 ob ol o:op_t)
+  : Lemma (requires distinct_ops ob ol /\ Fst_then_snd? (rc ob ol) /\
+                    get_rid o <> get_rid ol (*o,ol must be concurrent*) /\
+                    get_rid o1 <> get_rid ob /\ get_rid o <> get_rid o1 /\ //EXTRA!!
+                    ((~ (commutes_with o ob)) \/ Fst_then_snd? (rc o ol) \/ (Ts_order? (rc o ol) /\ fst o < fst ol)) /\
+                    eq (merge (do l ol) (do (do s1 ol) o1) (do (do s2 ob) ol) ) (do (do (do s3 ob) ol) o1))
+          (ensures eq (merge (do l ol) (do (do s1 ol) o1) (do (do (do s2 o) ob) ol)) (do (do (do (do s3 o) ob) ol) o1)) = ()
+
+let one_op_inter_right'2_base (l s1 s2 s3:concrete_st) (o1 ob ol o:op_t)
+  : Lemma (requires distinct_ops ob ol /\ Ts_order? (rc ob ol) /\
+                    get_rid o <> get_rid ol (*o,ol must be concurrent*) /\
+                    get_rid o1 <> get_rid ob /\ get_rid o <> get_rid o1 /\ //EXTRA!!
+                    (Either? (rc ob o1) \/ lo ob o1) /\
+                    //(Either? (rc o o1) \/ lo o o1) /\
+                    //(Either? (rc ol o1) \/ lo ol o1) /\
+                    ((~ (commutes_with o ob)) \/ Fst_then_snd? (rc o ol) \/ (Ts_order? (rc o ol) /\ fst o < fst ol)) /\
+                    eq (merge (do l ol) (do (do s1 ol) o1) (do (do s2 ob) ol) ) (do (do (do s3 ob) ol) o1))
+          (ensures eq (merge (do l ol) (do (do l ol) o1) (do (do (do l o) ob) ol)) (do (do (do (do l o) ob) ol) o1)) = ()
+
+let one_op_inter_right'2 (l s1 s2 s3:concrete_st) (o1 ob ol o:op_t)
+  : Lemma (requires distinct_ops ob ol /\ Ts_order? (rc ob ol) /\ fst ob < fst ol /\ get_rid ob <> get_rid ol /\ 
+                    get_rid o <> get_rid ol (*o,ol must be concurrent*) /\
+                    get_rid o1 <> get_rid ob /\ get_rid o1 <> get_rid o /\
+                    (Either? (rc o o1) \/ lo o o1) /\
+                    (forall o2. ((Either? (rc o1 o2) \/ lo o1 o2) /\ get_rid o1 <> get_rid o2) ==> eq (merge (do l ol) (do (do s1 ol) o1) (do (do (do s2 ob) ol) o2)) (do (do (do (do s3 ob) ol) o1) o2)) /\ //rc_inter_right
+                    (~ (Either? (rc o ob)) \/ Fst_then_snd? (rc o ol) \/ (Ts_order? (rc o ol) /\ fst o < fst ol)) /\
+                    eq (merge (do l ol) (do (do s1 ol) o1) (do (do s2 ob) ol) ) (do (do (do s3 ob) ol) o1))
+          (ensures eq_e (snd (merge (do l ol) (do (do s1 ol) o1) (do (do (do s2 o) ob) ol))) (snd (do (do (do (do s3 o) ob) ol) o1))) = ()
+
+(*let one_op_inter_right'1 (l s1 s2 s3:concrete_st) (o1 ob ol o:op_t)
   : Lemma (requires distinct_ops ob ol /\ Fst_then_snd? (rc ob ol) /\
                     get_rid o <> get_rid ol (*o,ol must be concurrent*) /\
                     ((~ (commutes_with o ob)) \/ Fst_then_snd? (rc o ol) \/ (Ts_order? (rc o ol) /\ fst o < fst ol)) /\
@@ -694,8 +766,35 @@ let one_op_inter_left' (l s1 s2 s3:concrete_st) (o1 ob ol o:op_t)
                     eq (merge (do l ol) (do (do s1 ob) ol) (do (do s2 ol) o1)) (do (do (do s3 ob) ol) o1))
           (ensures eq (merge (do l ol) (do (do (do s1 o) ob) ol) (do (do s2 ol) o1)) (do (do (do (do s3 o) ob) ol) o1)) = 
   if Fst_then_snd? (rc ob ol) then one_op_inter_left'1 l s1 s2 s3 o1 ob ol o 
-  else one_op_inter_left'2 l s1 s2 s3 o1 ob ol o
+  else one_op_inter_left'2 l s1 s2 s3 o1 ob ol o*)
 
+let one_op_inter_left'1 (l s1 s2 s3:concrete_st) (o1 ob ol o:op_t)
+  : Lemma (requires distinct_ops ob ol /\ Fst_then_snd? (rc ob ol) /\
+                    get_rid o <> get_rid ol (*o,ol must be concurrent*) /\
+                    get_rid o1 <> get_rid ob /\ get_rid o <> get_rid o1 /\ //EXTRA!!
+                    ((~ (commutes_with o ob)) \/ Fst_then_snd? (rc o ol) \/ (Ts_order? (rc o ol) /\ fst o < fst ol)) /\
+                    eq (merge (do l ol) (do (do s1 ob) ol) (do (do s2 ol) o1)) (do (do (do s3 ob) ol) o1))
+          (ensures eq (merge (do l ol) (do (do (do s1 o) ob) ol) (do (do s2 ol) o1)) (do (do (do (do s3 o) ob) ol) o1)) = ()
+
+let one_op_inter_left'2 (l s1 s2 s3:concrete_st) (o1 ob ol o:op_t)
+  : Lemma (requires distinct_ops ob ol /\ Ts_order? (rc ob ol) /\
+                    get_rid o <> get_rid ol (*o,ol must be concurrent*) /\
+                    get_rid o1 <> get_rid ob /\ get_rid o <> get_rid o1 /\ //EXTRA!!
+                    ((~ (commutes_with o ob)) \/ Fst_then_snd? (rc o ol) \/ (Ts_order? (rc o ol) /\ fst o < fst ol)) /\
+                    eq (merge (do l ol) (do (do s1 ob) ol) (do (do s2 ol) o1)) (do (do (do s3 ob) ol) o1))
+          (ensures eq (merge (do l ol) (do (do (do s1 o) ob) ol) (do (do s2 ol) o1)) (do (do (do (do s3 o) ob) ol) o1)) = admit()
+
+let one_op_inter_left'2_mod (l s1 s2 s3:concrete_st) (o1 ob ol o:op_t)
+  : Lemma (requires distinct_ops ob ol /\ Ts_order? (rc ob ol)  /\ fst ob < fst ol /\ get_rid ob <> get_rid ol /\ 
+                    get_rid o <> get_rid ol (*o,ol must be concurrent*) /\
+                    get_rid o1 <> get_rid ob /\ get_rid o <> get_rid o1 /\ //EXTRA!!
+                    (Either? (rc o o1) \/ lo o o1) /\
+                    (forall o2. ((Either? (rc o1 o2) \/ lo o1 o2) /\ get_rid o1 <> get_rid o2) ==> eq (merge (do l ol) (do (do (do s1 ob) ol) o2) (do (do s2 ol) o1)) (do (do (do (do s3 ob) ol) o1) o2)) /\ //rc_inter_right
+                    (~ (Either? (rc o ob)) \/ Fst_then_snd? (rc o ol) \/ (Ts_order? (rc o ol) /\ fst o < fst ol)) /\
+                    eq (merge (do l ol) (do (do s1 ob) ol) (do (do s2 ol) o1)) (do (do (do s3 ob) ol) o1))
+          (ensures eq_e (snd (merge (do l ol) (do (do (do s1 o) ob) ol) (do (do s2 ol) o1))) (snd (do (do (do (do s3 o) ob) ol) o1))) = 
+  one_op_inter_right'2 l s2 s1 s3 o1 ob ol o
+          
 // In general, the events ol,oi, below should be such that these exists o, (rc o ol), (rc o oi)
 let one_op_inter_lca' (l s1 s2 s3:concrete_st) (o1 ol oi:op_t)
   : Lemma (requires (exists o. Fst_then_snd? (rc o ol) \/ (Ts_order? (rc o ol) /\ fst o < fst ol)) /\ 
@@ -723,7 +822,7 @@ let zero_op_inter_base_left' (l s1 s2 s3:concrete_st) (ob ol:op_t)
                     eq (merge l (do s1 ob) (do s2 ol)) (do (do s3 ob) ol)) //***EXTRA***
           (ensures eq (merge (do l ol) (do (do s1 ob) ol) (do s2 ol)) (do (do s3 ob) ol)) = ()
 
-let zero_op_inter_right_l (l s1 s2 s3:concrete_st_l) (ob ol o:(nat & (nat & op_l)))
+(*let zero_op_inter_right_l (l s1 s2 s3:concrete_st_l) (ob ol o:(nat & (nat & op_l)))
   : Lemma (requires eq_l (merge_l (do_l l ol) (do_l s1 ol) (do_l (do_l s2 ob) ol)) (do_l (do_l s3 ob) ol))
           (ensures eq_l (merge_l (do_l l ol) (do_l s1 ol) (do_l (do_l (do_l s2 o) ob) ol)) (do_l (do_l (do_l s3 o) ob) ol)) = ()
 
@@ -756,9 +855,24 @@ let zero_op_inter_right' (l s1 s2 s3:concrete_st) (ob ol o:op_t)
   zero_op_inter_right_l (fst l) (fst s1) (fst s2) (fst s3) (get_op_l ob) (get_op_l ol) (get_op_l o);
   if Fst_then_snd? (rc ob ol) then
     zero_op_inter_right_e1 (snd l) (snd s1) (snd s2) (snd s3) (get_op_e ob) (get_op_e ol) (get_op_e o)
-  else zero_op_inter_right_e2 (snd l) (snd s1) (snd s2) (snd s3) (get_op_e ob) (get_op_e ol) (get_op_e o)
+  else zero_op_inter_right_e2 (snd l) (snd s1) (snd s2) (snd s3) (get_op_e ob) (get_op_e ol) (get_op_e o)*)
 
-let zero_op_inter_left_e1 (l s1 s2 s3:concrete_st_e) (ob ol o:(nat & (nat & op_e)))
+let zero_op_inter_right'1 (l s1 s2 s3:concrete_st) (ob ol o:op_t)
+  : Lemma (requires distinct_ops ob ol /\ Fst_then_snd? (rc ob ol) /\
+                    //get_rid o <> get_rid ol (*o,ol must be concurrent*) /\
+                    ((~ (commutes_with o ob)) \/ Fst_then_snd? (rc o ol) \/ (Ts_order? (rc o ol) /\ fst o < fst ol)) /\
+                    eq (merge (do l ol) (do s1 ol) (do (do s2 ob) ol)) (do (do s3 ob) ol))
+          (ensures eq (merge (do l ol) (do s1 ol) (do (do (do s2 o) ob) ol)) (do (do (do s3 o) ob) ol)) = ()
+
+let zero_op_inter_right'2 (l s1 s2 s3:concrete_st) (ob ol o:op_t)
+  : Lemma (requires distinct_ops ob ol /\ Ts_order? (rc ob ol) /\
+                    get_rid o <> get_rid ol (*o,ol must be concurrent*) /\
+                    eq (merge (do l ol) (do s1 ol) (do (do (do s2 ob) ol) o)) (do (do (do s3 ob) ol) o) /\ //EXTRA!! comes from one_op_inter_base_right'
+                    ((~ (commutes_with o ob)) \/ Fst_then_snd? (rc o ol) \/ (Ts_order? (rc o ol) /\ fst o < fst ol)) /\
+                    eq (merge (do l ol) (do s1 ol) (do (do s2 ob) ol)) (do (do s3 ob) ol))
+          (ensures eq (merge (do l ol) (do s1 ol) (do (do (do s2 o) ob) ol)) (do (do (do s3 o) ob) ol)) = ()
+          
+(*let zero_op_inter_left_e1 (l s1 s2 s3:concrete_st_e) (ob ol o:(nat & (nat & op_e)))
   : Lemma (requires Fst_then_snd? (rc_e ob ol) /\
                     //get_rid o <> get_rid ol (*o,ol must be concurrent*) /\
                     (((Disable? (snd (snd o)) /\ Enable? (snd (snd ob))) \/ (Enable? (snd (snd o)) /\ Disable? (snd (snd ob))) \/
@@ -789,7 +903,22 @@ let zero_op_inter_left' (l s1 s2 s3:concrete_st) (ob ol o:op_t)
           (ensures eq (merge (do l ol) (do (do (do s1 o) ob) ol) (do s2 ol)) (do (do (do s3 o) ob) ol)) = 
   if Fst_then_snd? (rc ob ol) then
     zero_op_inter_left_e1 (snd l) (snd s1) (snd s2) (snd s3) (get_op_e ob) (get_op_e ol) (get_op_e o)
-  else zero_op_inter_left_e2 (snd l) (snd s1) (snd s2) (snd s3) (get_op_e ob) (get_op_e ol) (get_op_e o)
+  else zero_op_inter_left_e2 (snd l) (snd s1) (snd s2) (snd s3) (get_op_e ob) (get_op_e ol) (get_op_e o)*)
+
+let zero_op_inter_left'1 (l s1 s2 s3:concrete_st) (ob ol o:op_t)
+  : Lemma (requires distinct_ops ob ol /\ Fst_then_snd? (rc ob ol) /\
+                    //get_rid o <> get_rid ol (*o,ol must be concurrent*) /\
+                    ((~ (commutes_with o ob)) \/ Fst_then_snd? (rc o ol) \/ (Ts_order? (rc o ol) /\ fst o < fst ol)) /\
+                    eq (merge (do l ol) (do (do s1 ob) ol) (do s2 ol)) (do (do s3 ob) ol))
+          (ensures eq (merge (do l ol) (do (do (do s1 o) ob) ol) (do s2 ol)) (do (do (do s3 o) ob) ol)) = ()
+
+let zero_op_inter_left'2 (l s1 s2 s3:concrete_st) (ob ol o:op_t)
+  : Lemma (requires distinct_ops ob ol /\ Ts_order? (rc ob ol) /\
+                    get_rid o <> get_rid ol (*o,ol must be concurrent*) /\
+                    eq (merge (do l ol) (do (do (do s1 ob) ol) o) (do s2 ol)) (do (do (do s3 ob) ol) o) /\ //EXTRA!!
+                    ((~ (commutes_with o ob)) \/ Fst_then_snd? (rc o ol) \/ (Ts_order? (rc o ol) /\ fst o < fst ol)) /\
+                    eq (merge (do l ol) (do (do s1 ob) ol) (do s2 ol)) (do (do s3 ob) ol))
+          (ensures eq (merge (do l ol) (do (do (do s1 o) ob) ol) (do s2 ol)) (do (do (do s3 o) ob) ol)) = ()
 
 // In general, the event "ol" below should be such that these exists o', (rc o' ol)
 let zero_op_inter_lca_v1' (l s1 s2 s3:concrete_st) (ol:op_t)
